src/program_proof/reconnectclient/proof.v
@@ -7,11 +7,129 @@ Section proof.
 Context `{!heapGS Σ}.
 Context `{!urpcregG Σ}.
 
-Definition is_ReconnectingClient : loc → u64 → iProp Σ.
-Admitted.
+Definition own_ReconnectingClient ck host mu : iProp Σ :=
+  ∃ (valid:bool) (urpcCl:loc) (making:bool) (made_cond:loc),
+  "Hvalid" ∷ ck ↦[ReconnectingClient :: "valid"] #valid ∗
+  "HurpcCl" ∷ ck ↦[ReconnectingClient :: "urpcCl"] #urpcCl ∗
+  "#Hcl" ∷ □(if valid then is_uRPCClient urpcCl host else True) ∗
+  "Hmaking" ∷ ck ↦[ReconnectingClient :: "making"] #making ∗
+  "Hmade_cond" ∷ ck ↦[ReconnectingClient :: "made_cond"] #made_cond ∗
+  "#Hmade_cond_cond" ∷ is_cond made_cond mu
+.
 
-Global Instance is_ReconnectingClient_pers cl host : Persistent (is_ReconnectingClient cl host).
-Admitted.
+Definition reconnectN := nroot .@ "reconnect".
+
+Definition is_ReconnectingClient ck (host:u64) : iProp Σ :=
+  ∃ mu,
+    "#Haddr" ∷ readonly (ck ↦[ReconnectingClient :: "addr"] #host) ∗
+    "#Hmu" ∷ readonly (ck ↦[ReconnectingClient :: "mu"] mu) ∗
+    "#HmuInv" ∷ is_lock reconnectN mu (own_ReconnectingClient ck host mu)
+.
+
+Lemma wp_getClient ck host :
+  {{{
+       is_ReconnectingClient ck host
+  }}}
+   ReconnectingClient__getClient #ck
+  {{{
+       urpcCl, RET #urpcCl; is_uRPCClient urpcCl host
+  }}}
+.
+Proof.
+  iIntros (Φ) "#His HΦ".
+  iNamed "His".
+  wp_call.
+  wp_loadField.
+  wp_apply (acquire_spec with "HmuInv").
+  iIntros "[Hlocked Hown]".
+  iNamed "Hown".
+  wp_pures.
+  wp_loadField.
+  wp_if_destruct.
+  { (* there's already a client there *)
+    wp_loadField.
+    wp_loadField.
+    wp_apply (release_spec with "[- HΦ]").
+    { iFrame "HmuInv ∗".
+      repeat iExists _.
+      iFrame "∗#".
+    }
+    wp_pures.
+    by iApply "HΦ".
+  }
+  (* else make a new one *)
+  wp_storeField.
+  wp_loadField.
+  wp_apply (release_spec with "[- HΦ]").
+  { iFrame "HmuInv ∗".
+    repeat iExists _.
+    iFrame "∗#".
+  }
+  wp_pures.
+  wp_apply (wp_ref_of_zero).
+  { done. }
+  wp_pures.
+  iIntros (newRpcCl) "HnewRpcCl".
+  wp_pures.
+
+  iAssert (∃ (cl_ptr:loc), "HnewRpcCl" ∷ newRpcCl ↦[ptrT] #cl_ptr)%I with "[HnewRpcCl]" as "HH".
+  { iExists _; iFrame. }
+  wp_forBreak.
+  wp_pures.
+  wp_apply (wp_ref_of_zero).
+  { done. }
+  iIntros (err_ptr) "Herr".
+  wp_pures.
+  wp_loadField.
+  wp_apply (wp_TryMakeClient).
+  iIntros (??) "Hnewcl".
+  wp_pures.
+  wp_store.
+  iNamed "HH".
+  wp_store.
+  wp_load.
+  wp_if_destruct.
+  {
+    destruct (decide _); last by exfalso.
+    iRight.
+    iModIntro.
+    iSplitR; first done.
+    iDestruct "Hnewcl" as "#Hnewcl".
+    wp_pures.
+    wp_loadField.
+    wp_apply (acquire_spec with "HmuInv").
+    iIntros "[Hlocked Hown]".
+    iNamed "Hown".
+    wp_pures.
+    wp_load.
+    wp_storeField.
+    iClear "Hcl Hmade_cond_cond".
+    iNamed "Hown".
+    wp_loadField.
+    wp_apply (wp_condBroadcast with "Hmade_cond_cond").
+    wp_pures.
+    wp_storeField.
+    wp_storeField.
+    wp_loadField.
+    wp_apply (release_spec with "[- HΦ HnewRpcCl]").
+    { iFrame "HmuInv ∗".
+      repeat iExists _.
+      iFrame "∗#".
+    }
+    wp_pures.
+    wp_load.
+    by iApply "HΦ".
+  }
+  {
+    wp_apply wp_Sleep.
+    wp_pures.
+    iLeft.
+    iModIntro.
+    iSplitR; first done.
+    iFrame.
+    iExists _; iFrame.
+  }
+Qed.
 
 Lemma wp_ReconnectingClient__Call2 γsmap (cl_ptr:loc) (rpcid:u64) (host:u64) req rep_out_ptr
       (timeout_ms : u64) dummy_sl_val (reqData:list u8) Spec Φ :
@@ -33,7 +151,62 @@ Lemma wp_ReconnectingClient__Call2 γsmap (cl_ptr:loc) (rpcid:u64) (host:u64) re
   ) -∗
   WP ReconnectingClient__Call #cl_ptr #rpcid (slice_val req) #rep_out_ptr #timeout_ms {{ Φ }}.
 Proof.
-Admitted.
+  iIntros "#Hre #? Hsl Hrep #? HΦerr".
+  iIntros.
+  wp_call.
+  wp_apply (wp_getClient with "[$]").
+  iIntros.
+  wp_pures.
+  wp_apply (wp_Client__Call with "[$] [$Hsl $Hrep]").
+  { iFrame "#". }
+  iIntros (?) "(? & Hsl & HΦ)".
+  wp_pures.
+  wp_if_destruct.
+  {
+    iNamed "Hre".
+    wp_loadField.
+    wp_apply (acquire_spec with "HmuInv").
+    iIntros "[Hlocked Hown]".
+    iNamed "Hown".
+    wp_pures.
+    wp_storeField.
+    wp_loadField.
+    wp_apply (release_spec with "[Hlocked Hvalid Hmaking HurpcCl Hmade_cond]").
+    {
+      iFrame "HmuInv Hlocked".
+      iNext. repeat iExists _.
+      iFrame "∗#".
+      done.
+    }
+    wp_pures.
+    rewrite Heqb.
+    iModIntro.
+    destruct err.
+    {
+     iApply ("HΦerr" with "[] Hsl [-]").
+     { done. }
+     { iFrame. }
+    }
+    {
+      exfalso. done.
+    }
+  }
+  wp_pures.
+  destruct err.
+  {
+   iApply ("HΦerr" with "[] Hsl").
+   { iPureIntro. simpl. by destruct c. }
+   iFrame.
+   done.
+  }
+  {
+   simpl.
+   iDestruct "HΦ" as (??) "(Hrep & Hsl2 & HΦ)".
+   iApply ("HΦ" with "Hsl Hrep").
+   iFrame.
+   done.
+  }
+Qed.
 
 Lemma wp_MakeReconnectingClient (srv:u64):
   {{{
@@ -44,6 +217,34 @@ Lemma wp_MakeReconnectingClient (srv:u64):
        (cl_ptr:loc), RET #cl_ptr; is_ReconnectingClient cl_ptr srv
   }}}.
 Proof.
-Admitted.
+  iIntros (Φ) "_ HΦ".
+  wp_lam.
+  wp_apply (wp_allocStruct).
+  { repeat econstructor. }
+  iIntros (?) "Hl".
+  iDestruct (struct_fields_split with "Hl") as "HH".
+  iNamed "HH".
+  wp_pures.
+  wp_apply (wp_new_free_lock).
+  iIntros (?) "HmuInv".
+  wp_storeField.
+  wp_storeField.
+  wp_storeField.
+  wp_loadField.
+  wp_apply (wp_newCond' with "HmuInv").
+  iIntros (?) "[HmuInv #Hcond]".
+  wp_storeField.
+  wp_storeField.
+  iApply "HΦ".
+  iMod (readonly_alloc_1 with "mu") as "#Hmu".
+  iMod (readonly_alloc_1 with "addr") as "#Haddr".
+  iExists _.
+  iFrame "#".
+  iMod (alloc_lock with "HmuInv [-]") as "$"; last done.
+  iNext.
+  repeat iExists _.
+  iFrame "∗#".
+  done.
+Qed.
 
 End proof.
